internal/Notations.v
@@ -1,6 +1,7 @@
 Reserved Notation "x ‘‘→’’ y" (at level 99, right associativity, y at level 200).
 Reserved Notation "x ‘→’ y" (at level 99, right associativity, y at level 200).
 Reserved Notation "x ‘→'’ y" (at level 99, right associativity, y at level 200).
+Reserved Notation "x ‘‘→'’’ y" (at level 99, right associativity, y at level 200).
 Reserved Notation "x ‘’ y" (at level 15, left associativity).
 Reserved Notation "x ‘’₀ y" (at level 15, left associativity).
 Reserved Notation "x ‘’₁ y" (at level 15, left associativity).
@@ -24,6 +25,9 @@ Reserved Notation "Γ ‘▻’ x" (at level 65, left associativity).
 Reserved Notation "Γ ‘▻▻’ Γ'" (at level 65, left associativity).
 Reserved Notation "□ T" (at level 0).
 Reserved Notation "x [ 0 ↦ y ]" (at level 0, no associativity).
+Reserved Infix "∘" (at level 40, left associativity).
+Reserved Infix "‘∘’" (at level 40, left associativity).
+Reserved Infix "‘‘∘’’" (at level 40, left associativity).
 Notation "( x ; y )" := (existT _ x y).
 Notation "x .1" := (projT1 x) (at level 3, format "x '.1'").
 Notation "x .2" := (projT2 x) (at level 3, format "x '.2'").
